examples/stateful_bignum/shift_st.fst
@@ -1,0 +1,150 @@
+module Shift
+
+
+open Heap
+open ST
+open IntLib
+open Bigint
+open Eval
+
+type norm_bigint = a:bigint{ forall (i:nat). Bigint63.t a i = Bigint63.t a 0 }
+
+val shift:
+  a:bigint -> offset:nat ->
+  ST bigint
+     (requires (fun h -> 
+		(inHeap h a)
+		/\ (getLength h a > 0)
+     ))
+     (ensures (fun h0 b h1 ->
+	       (inHeap h1 b)
+	       /\ (inHeap h0 a)
+	       /\ (modifies !{} h0 h1)
+	       /\ (getLength h1 b = getLength h0 a + offset)
+	       /\ (forall (i:nat).
+		   (i < getLength h0 a ==> (getValue h1 b (i+offset) = getValue h0 a i
+                                         /\ getSize h1 b (i+offset) = getSize h0 a i))
+		   /\ (i < offset ==> (getValue h1 b i = 0 /\ getSize h1 b i = 0)))
+	       /\ (eval h1 b (getLength h1 b) = pow2 (offset * (Bigint63.t a 0)) * eval h0 a (getLength h0 a))
+     ))
+let shift a offset =
+  let res = Bigint.mk_zero_bigint (get_length a + offset) in
+  Array.blit a 0 res offset (get_length a);
+  Bigint63.data a := res
+
+(* How to make it constant time ? *)
+val shift_by_bits_aux:
+  a:bigint -> bits:nat -> b:bigint -> len:nat ->
+  ST unit
+     (requires (fun h ->
+		(inHeap h a)
+		/\ (inHeap h b)
+		/\ (SameFormat h h a b)
+		/\ (len <= getLength h0 a)
+		/\ (forall (i:nat). (i >= len /\ i < getLength h0 a)
+		    ==> (getSize h0 b i = getSize h0 a i + bits 
+                        /\ getValue h0 b i = pow2 bits * getValue h0 a i))
+		/\ (forall (i:nat). i < len
+		    ==> getSize a i <= wordSize a - bits)
+     ))
+     (ensures (fun h0 u h1 ->
+	       (inHeap h0 a)
+	       /\ (inHeap h0 b)
+	       /\ (SameFormat h0 h0 a b)
+	       /\ (modifies !{Bigint63.data b} h0 h1)
+	       /\ (SameFormat h0 h1 b b)
+	       /\ (forall (i:nat). i < getLength h0 a 
+		   ==> (getSize h0 b i = getSize h0 a i + bits 
+		       /\ getValue h0 b i = pow2 bits * getValue h0 a i))
+     ))
+let rec shift_by_bits_aux a bits b len =
+  match len with
+  | 0 -> ()
+  | _ ->
+     let i = len - 1 in
+     let h0 = 
+       erase (ST.get()) in
+     let v = Bigint.mk_tint b (getSize h0 a i + bits) (shift_left (get a i)) in
+     Bigint.updateBigint b i v;
+     shift_by_bits_aux a bits b (len-1)
+
+val shift_by_bits : 
+  a:bigint -> bits:nat -> 
+  ST bigint
+     (requires (fun h -> 
+		(inHeap h a)
+		/\ (maxSize h a < wordSize a - bits)
+     ))
+     (ensures (fun h0 b h1 ->
+	       (inHeap h0 a)
+	       /\ (inHeap h1 b)
+	       /\ (modifies !{} h0 h1)
+	       /\ (eval h1 b (getLength h1 b) = pow2 bits * eval h0 a (getLength h0 a))
+	       /\ (forall (i:nat). i < getLength h1 b
+		   ==> (getValue h1 b = pow2 bits * getValue h0 a /\ getSize h1 b = bits + getSize h0 a))
+     ))
+let shift_by_bits a bits =
+  let b = Bigint63.data (Bigint.mk_zero_bigint (get_length a)) (Bigint63.t a) in
+  shift_by_bits_aux a bits b (get_length a)
+	
+val shift_over_by_bits_aux :
+  a:norm_bigint -> bits:nat -> b:norm_bigint -> len:nat -> 
+  ST norm_bigint 
+     (requires (fun h -> 
+		(inHeap h a)
+		/\ (inHeap h b)
+		/\ (Normalized h a)
+		/\ (Normalized h b)
+		/\ (getLength h b = getLength h a + 1)
+		/\ (forall (i:nat). i < getLength h a 
+		    ==> bits < Bigint63.t a i)
+		/\ (eval h b (i+1) = pow2 bits * eval h a i)
+     ))
+     (ensures (fun h0 u h1 ->
+	       (inHeap h0 a)
+	       /\ (inHeap h0 b)
+	       /\ (modifies !{Bigint63.data b} h0 h1)
+	       /\ (getLength h0 b = getLength h0 a + 1)
+	       /\ (getLength h1 b = getLength h0 b)
+	       /\ (forall (i:nat). i < getLength h0 a 
+		   ==> bits < Bigint63.t a i)
+	       /\ (eval h1 b (getLength h1 b) = pow2 bits * eval h0 a (getLength h0 a))
+	       /\ (Normalized h1 b)
+     ))
+let shift_over_by_bits_aux a bits b len =
+  match get_length a - len with
+  | 0 -> ()
+  | _ ->
+     let i = len in
+     let ai = get a i in
+     let modulus = (Bigint63.t a i - pow2 bits)
+     let carry = div ai modulus in (* Redundant recursives calls, put in variable *)
+     let remainder = shift_left (signed_modulo a modulus) bits in
+     let carry = Bigint.mk_tint a (Bigint63.t a i) carry in
+     let remainder = Bigint.mk_tint a (Bigint63.t a i) remainder in
+     Bigint.updateBigint b (i+1) carry;
+     Bigint.updateBigint b i remainder;
+     shift_over_by_bits_aux a bits b (i+1)
+     
+val shift_over_by_bits :
+  a:norm_bigint -> bits:nat ->
+  ST norm_bigint 
+     (requires (fun h -> 
+		(inHeap h a)
+		/\ (Normalized h a)
+		/\ (forall (i:nat). i < getLength h a 
+		    ==> bits < Bigint63.t a i)
+     ))
+     (ensures (fun h0 b h1 ->
+	       (inHeap h0 a)
+	       /\ (inHeap h1 b)
+	       /\ (modifies !{} h0 h1)
+	       /\ (forall (i:nat). i < getLength h0 a 
+		   ==> bits < Bigint63.t a i)
+	       /\ (eval h1 b (getLength h1 b) = pow2 bits * eval h0 a (getLength h0 a))
+	       /\ (Normalized h1 b)
+     ))
+let shift_over_by_bits a bits =
+  let b = Bigint63.data (Bigint.mk_zero_bigint (get_length a + 1)) (Bigint63.t a) in
+  shift_over_by_bits_aux a bits b (get_length a)
+		       
